[llir-semantics] Helpers for LLIR lowering

test/fibonacci.c
@@ -1,0 +1,9 @@
+unsigned fib(unsigned n) {
+  unsigned a = 0, b = 1;
+  while (n--) {
+    unsigned c = a + b;
+    a = b;
+    b = c;
+  }
+  return b;
+}
