Dom.v
@@ -16,17 +16,11 @@ Section FUNCTION.
 
   Definition entry: node := f.(fn_entry).
 
-  Definition Succ (from: node) (to: node) :=
-    match PTrie.get f.(fn_insts) from with
-    | Some i => SuccessorOfInst i to
-    | None => False
-    end.
-
   Inductive Closure (x: node): node -> Prop :=
     | closure_refl:
       Closure x x
     | closure_step:
-      forall (y: node) (STEP: Succ x y),
+      forall (y: node) (STEP: SuccOf f x y),
         Closure x y
     | closure_trans:
       forall (y: node) (z: node),
@@ -38,7 +32,7 @@ Section FUNCTION.
       Reachable f.(fn_entry)
     | reach_succ:
       forall (a: node) (b: node)
-        (HD: Succ a b)
+        (HD: SuccOf f a b)
         (TL: Reachable a),
         Reachable b
     .
@@ -47,9 +41,7 @@ Section FUNCTION.
     forall (n: node) (m:node),
       Reachable n -> Closure n m -> Reachable m.
   Proof.
-    intros n m.
-    intro HreachN.
-    intro Hclosure.
+    intros n m HreachN Hclosure.
     induction Hclosure.
     - apply HreachN.
     - apply (reach_succ x). apply STEP. apply HreachN.
@@ -62,10 +54,11 @@ Section FUNCTION.
     | path_nil:
       forall (n: node)
         (REACH: Reachable n),
-        Path n nil n
+        Path n [] n
     | path_cons:
       forall (from: node) (next: node) (to: node) (p: list node)
-        (HD: Succ from next)
+        (REACH: Reachable from)
+        (HD: SuccOf f from next)
         (TL: Path next p to),
         Path from (from :: p) to
     .
@@ -80,8 +73,63 @@ Section FUNCTION.
     - simpl. inversion Hxy. apply Hyz.
     - rewrite <- app_comm_cons.
       inversion Hxy.
-      apply (path_cons a next). apply HD.
+      apply (path_cons a next). apply REACH. apply HD.
       apply (IHxy yz next y z). apply TL. apply Hyz.
+  Qed.
+
+  Theorem path_app_inv:
+    forall (xy: list node) (yz: list node) (x: node) (z: node),
+      Path x (xy ++ yz) z ->
+        exists (y: node), Path x xy y /\ Path y yz z.
+  Proof.
+    induction xy; intros yz x z Hpath.
+    {
+      exists x.
+      split.
+      + apply path_nil. inversion Hpath; apply REACH.
+      + simpl in Hpath. apply Hpath.
+    }
+    {
+      inversion Hpath.
+      subst to a from.
+      generalize (IHxy yz next z TL). intros Hind.
+      destruct Hind as [y [Hl Hr]].
+      exists y.
+      split.
+      {
+        apply path_cons with (next := next).
+        + apply REACH.
+        + apply HD.
+        + apply Hl.
+      }
+      {
+        apply Hr.
+      }
+    }
+  Qed.
+
+  Theorem path_last:
+    forall (n: node) (m: node) (nm: list node),
+      n <> m -> Path n nm m -> 
+        exists (p: node) (np: list node),
+          nm = np ++ [p] /\ Path n np p /\ SuccOf f p m.
+  Proof.
+    intros n m nm Hne Hpath.
+    inversion Hpath. apply Hne in H1. inversion H1.
+    assert (Hneq: n :: p <> []). intros contra. inversion contra.
+    generalize (List.exists_last Hneq). intros Hlast.
+    destruct Hlast as [path' [p' Hlast]].
+    exists p'. exists path'.
+    assert (Hpath': Path n (path' ++ [p']) m).
+    { rewrite <- Hlast. rewrite H0. apply Hpath. }
+    generalize (path_app_inv path' [p'] n m Hpath'). intros Hstep.
+    destruct Hstep as [y [Hl Hr]].
+    inversion Hr.
+    subst y from from0 to to0 p0.
+    repeat split.
+    - apply Hlast.
+    - apply Hl.
+    - inversion TL0. subst next0 n0. apply HD0.
   Qed.
 
   Theorem path_next:
@@ -100,7 +148,7 @@ Section FUNCTION.
     {
       intros Hreach.
       exists [x].
-      apply (path_cons x y y). apply STEP. apply path_nil.
+      apply (path_cons x y y). apply Hreach. apply STEP. apply path_nil.
       apply (reach_succ x). apply STEP. apply Hreach.
     }
     {
@@ -140,8 +188,16 @@ Section FUNCTION.
     | dom_path:
       forall (a: node) (b: node)
         (PATH: forall (p: list node), Path entry p b -> In a p)
-        (REACH: Reachable a),
+        (REACH: Reachable b),
         Dominates a b
+    .
+
+  Inductive StrictlyDominates: node -> node -> Prop :=
+    | sdom_path:
+        forall (a: node) (b: node)
+          (DOM: Dominates a b)
+          (STRICT: a <> b),
+          StrictlyDominates a b
     .
 
   Theorem entry_dominates_all:
@@ -163,11 +219,11 @@ Section FUNCTION.
           + simpl. auto.
         }
         {
-          apply reach_entry.
+          apply Hreach.
         }
   Qed.
 
-  Theorem dominator_of_entry:
+  Theorem dom_of_entry:
     forall (n: node),
       Dominates n entry -> n = entry.
   Proof.
@@ -188,25 +244,71 @@ Section FUNCTION.
     }
   Qed.
 
+  Theorem dom_reaches:
+    forall (n: node),
+      Dominates entry n -> Reachable n.
+  Proof.
+    intros n Hdom.
+    inversion Hdom. apply reach_entry. apply REACH.
+  Qed.
+
+  Lemma sdom_not_dom: 
+    forall n m,
+      StrictlyDominates n m -> ~Dominates m n.
+  Admitted.
+
   Theorem dom_antisym:
     forall (n: node) (m: node),
       Dominates n m ->
       Dominates m n ->
       m = n.
-   Admitted.
+  Proof.
+    intros n m Hnm Hmn.
+    destruct (Pos.eq_dec m n) as [|Ene]. apply e.
+    apply sdom_not_dom in Hnm. inversion Hnm.
+    apply sdom_path. apply Hmn. apply Ene.
+  Qed.
 
   Theorem dom_trans:
     forall (n: node) (m: node) (p: node),
       Dominates n m -> Dominates m p -> Dominates n p.
   Admitted.
 
-  Inductive StrictlyDominates: node -> node -> Prop :=
-    | sdom_path:
-        forall (a: node) (b: node)
-          (DOM: Dominates a b)
-          (STRICT: a <> b),
-          StrictlyDominates a b
-    .
+  Theorem dom_step:
+    forall (n: node) (m: node),
+      Reachable n
+      /\
+      SuccOf f n m
+      /\
+      entry <> m
+      /\
+      (forall (n': node), SuccOf f n' m -> n = n') ->
+      Dominates n m.
+  Proof.
+    intros n m [Hreach [Hsucc [Hne Huniq]]].
+    destruct (Pos.eq_dec n m). subst n. apply dom_self.
+    apply dom_path.
+    {
+      intros path Hpath.
+      inversion Hpath.
+      {
+        subst.
+        assert (entry = entry). reflexivity. apply Hne in H. inversion H.
+      }
+      {
+        subst.
+        generalize (path_last entry m (entry :: p) Hne Hpath). intros Hsplit.
+        destruct Hsplit as [path [np [Hp [_ Hsucc']]]].
+        rewrite Hp.
+        apply in_or_app.
+        right. left. symmetry.
+        apply Huniq. apply Hsucc'.
+      }
+    }
+    {
+      apply reach_succ with (a := n). apply Hsucc. apply Hreach.
+    }
+  Qed.
 
   Theorem sdom_trans:
     forall (n: node) (m: node) (p: node),
@@ -230,11 +332,70 @@ Section FUNCTION.
     apply STRICT.
     reflexivity.
   Qed.
+
+  Inductive BasicBlock: node -> node -> Prop :=
+    | block_header:
+      forall (header: node)
+        (REACH: Reachable header)
+        (TERM: header = entry \/ forall (term: node), SuccOf f term header -> TermAt f term),
+        BasicBlock header header
+    | block_elem:
+      forall (header: node) (prev: node) (elem: node)
+        (NOT_HEADER: header <> elem)
+        (NOT_ENTRY: entry <> elem)
+        (BLOCK: BasicBlock header prev)
+        (PRED: SuccOf f prev elem)
+        (NOPHI: f.(fn_phis) ! elem = None)
+        (UNIQ: forall (prev': node), SuccOf f prev' elem -> prev' = prev),
+        BasicBlock header elem
+    .
+
+  Theorem bb_reaches:
+    forall (header: node) (elem: node),
+      BasicBlock header elem -> Reachable elem.
+  Proof.
+    intros header elem Hbb.
+    induction Hbb. apply REACH.
+    apply reach_succ with (a := prev); auto.
+  Qed.
+
+  Theorem bb_entry_header:
+    BasicBlock entry entry.
+  Proof.
+    apply block_header.
+    apply reach_entry.
+    left. reflexivity.
+  Qed.
+
+  Theorem bb_header_dom_nodes:
+    forall (header: node) (elem: node),
+      BasicBlock header elem -> Dominates header elem.
+  Proof.
+    intros header elem Hbb.
+    induction Hbb. apply dom_self.
+    apply dom_trans with (m := prev); auto.
+    apply dom_step.
+    repeat split.
+    + apply bb_reaches with (header := header). apply Hbb.
+    + apply PRED.
+    + apply NOT_ENTRY.
+    + intros n Hsucc. symmetry. apply UNIQ. apply Hsucc.
+  Qed.
+
+  Inductive BasicBlockSucc: node -> node -> Prop :=
+    | basic_block_succ:
+      forall (from: node) (to: node) (term: node)
+        (HDR_FROM: BasicBlock from term)
+        (HDR_TO: BasicBlock to to)
+        (SUCC: SuccOf f term to),
+        BasicBlockSucc from to
+    .
+
 End FUNCTION.
 
 Lemma eq_cfg_dom:
   forall (f: func) (f': func),
-    (forall (src: node) (dst: node), Succ f src dst <-> Succ f' src dst) ->
+    (forall (src: node) (dst: node), SuccOf f src dst <-> SuccOf f' src dst) ->
     forall (src: node) (dst: node),
       Dominates f src dst <-> 
       Dominates f' src dst.
