LLIR.v
@@ -9,22 +9,42 @@ Require Import LLIR.Maps.
 Require Import LLIR.State.
 Require Import LLIR.Values.
 
+Import ListNotations.
 
 
 Record object := mkobject
   { obj_size : positive
-  ; align: positive
+  ; obj_align: positive
   }.
+
+Inductive ty : Type :=
+  | I8
+  | I16
+  | I32
+  | I64
+  | I128
+  | F32
+  | F64
+  | F80
+  .
 
 Inductive unop : Type :=
   | LLSext
   | LLZext
+  | LLFext
+  | LLXext
   | LLTrunc
+  | LLNeg
   .
 
 Inductive binop : Type :=
   | LLAdd
   | LLSub
+  | LLMul
+  | LLUDiv
+  | LLSDiv
+  | LLURem
+  | LLSRem
   | LLCmp
   | LLSll
   | LLSra
@@ -32,25 +52,35 @@ Inductive binop : Type :=
   | LLXor
   | LLAnd
   | LLOr
+  | LLRotl
+  | LLUAddO
+  | LLUMulO
   .
 
 Inductive inst : Type :=
+  | LLInvoke (callee: reg) (args: list reg) (dst: reg) (next: node) (exn: option node)
   | LLLd (addr: reg) (dst: reg) (next: node)
   | LLSt (addr: reg) (val: reg) (next: node)
-  | LLArg (index: positive) (dst: reg) (next: node)
-  | LLConst (value: qword) (dst: reg) (next: node)
+  | LLArg (index: nat) (dst: reg) (next: node)
+  | LLInt8 (value: INT8.t) (dst: reg) (next: node)
+  | LLInt16 (value: INT16.t) (dst: reg) (next: node)
+  | LLInt32 (value: INT32.t) (dst: reg) (next: node)
+  | LLInt64 (value: INT64.t) (dst: reg) (next: node)
   | LLFrame (object: positive) (dst: reg) (next: node)
   | LLGlobal (object: positive) (dst: reg) (next: node)
   | LLExtern (id: positive) (next: node)
-  | LLInvoke (callee: reg) (args: list reg) (dst: reg) (next: node) (exn: node)
   | LLRet (value: reg)
+  | LLRetVoid
   | LLJcc (cond: reg) (bt: node) (bf: node)
   | LLJmp (target: node)
-  | LLUnop (op: unop) (arg: reg) (dst: reg) (next: node)
-  | LLBinop (op: binop) (lhs: reg) (rhs: reg) (dst: reg) (next: node)
+  | LLUndef (ty: ty) (dst: reg) (next: node)
+  | LLUnop (ty: ty) (op: unop) (arg: reg) (dst: reg) (next: node)
+  | LLBinop (ty: ty) (op: binop) (lhs: reg) (rhs: reg) (dst: reg) (next: node)
   .
 
-Inductive phi : Type := LLPhi : list reg -> reg -> phi.
+Inductive phi : Type :=
+  | LLPhi (ins: list (node * reg)) (dst: reg)
+  .
 
 Definition phis := list phi.
 
@@ -58,8 +88,7 @@ Definition inst_map := PTrie.t inst.
 Definition phi_map := PTrie.t phis.
 
 Record func : Type := mkfunc
-  { fn_args: positive
-  ; fn_stack: PTrie.t object
+  { fn_stack: PTrie.t object
   ; fn_insts: inst_map
   ; fn_phis: phi_map
   ; fn_entry: node
@@ -69,22 +98,26 @@ Record func : Type := mkfunc
 Definition prog : Type := PTrie.t func.
 
 
-
 Definition Defs (i: inst) (r: reg): Prop :=
   match i with
   | LLLd _ dst _ => dst = r
   | LLSt _ _ _ => False
   | LLArg _ dst _ => dst = r
-  | LLConst _ dst _ => dst = r
+  | LLInt8 _ dst _ => dst = r
+  | LLInt16 _ dst _ => dst = r
+  | LLInt32 _ dst _ => dst = r
+  | LLInt64 _ dst _ => dst = r
   | LLFrame _ dst _ => dst = r
   | LLGlobal _ dst _ => dst = r
   | LLExtern _ _ => False
   | LLInvoke _ _ dst _ _ => dst = r
   | LLRet _ => False
+  | LLRetVoid => False
   | LLJcc _ _ _ => False
   | LLJmp _ => False
-  | LLUnop _ _ dst _ => dst = r
-  | LLBinop _ _ _ dst _ => dst = r
+  | LLUndef _ dst _ => dst = r
+  | LLUnop _ _ _ dst _ => dst = r
+  | LLBinop _ _ _ _ dst _ => dst = r
   end.
 
 Definition Uses (i: inst) (r: reg): Prop :=
@@ -92,33 +125,65 @@ Definition Uses (i: inst) (r: reg): Prop :=
   | LLLd addr _ _ => addr = r
   | LLSt addr val _ => addr = r \/ val = r
   | LLArg _ _ _ => False
-  | LLConst _ _ _ => False
+  | LLInt8 _ _ _ => False
+  | LLInt16 _ _ _ => False
+  | LLInt32 _ _ _ => False
+  | LLInt64 _ _ _ => False
   | LLFrame _ _ _ => False
   | LLGlobal _ _ _ => False
   | LLExtern _ _ => False
   | LLInvoke callee args _ _ _ => callee = r \/ In r args
   | LLRet value => value = r
+  | LLRetVoid => False
   | LLJcc cond _ _ => cond = r
   | LLJmp _ => False
-  | LLUnop _ arg _ _ => arg = r
-  | LLBinop _ lhs rhs _ _ => lhs = r \/ rhs = r
+  | LLUndef _ _ _ => False
+  | LLUnop _ _ arg _ _ => arg = r
+  | LLBinop _ _ lhs rhs _ _ => lhs = r \/ rhs = r
   end.
 
-Definition SuccessorOfInst (i: inst) (succ: node): Prop :=
+Definition Succeeds (i: inst) (succ: node): Prop :=
   match i with
   | LLLd _ _ next => next = succ
   | LLSt _ _ next => next = succ
   | LLArg _ _ next => next = succ
-  | LLConst _ _ next => next = succ
+  | LLInt8 _ _ next => next = succ
+  | LLInt16 _ _ next => next = succ
+  | LLInt32 _ _ next => next = succ
+  | LLInt64 _ _ next => next = succ
   | LLFrame _ _ next => next = succ
   | LLGlobal _ _ next => next = succ
   | LLExtern _ next => next = succ
-  | LLInvoke _ _ _ next exn => next = succ \/ exn = succ
+  | LLInvoke _ _ _ next exn => next = succ \/ exn = Some succ
   | LLRet _ => False
+  | LLRetVoid => False
   | LLJcc _ bt bf => bt = succ \/ bf = succ
   | LLJmp target => target = succ
-  | LLUnop _ _ _ next => next = succ
-  | LLBinop _ _ _ _ next => next = succ
+  | LLUndef _ _ next => next = succ
+  | LLUnop _ _ _ _ next => next = succ
+  | LLBinop _ _ _ _ _ next => next = succ
+  end.
+
+Definition Terminator (i: inst): Prop :=
+  match i with
+  | LLInvoke _ _ _ _ _ => True
+  | LLRet _ => True
+  | LLRetVoid => True
+  | LLJcc _ _ _ => True
+  | LLJmp _ => True
+  | LLLd _ _ _ => False
+  | LLSt _ _ _ => False
+  | LLArg _ _ _ => False
+  | LLInt8 _ _ _ => False
+  | LLInt16 _ _ _ => False
+  | LLInt32 _ _ _ => False
+  | LLInt64 _ _ _ => False
+  | LLFrame _ _ _ => False
+  | LLGlobal _ _ _ => False
+  | LLExtern _ _ => False
+  | LLUndef _ _ _ => False
+  | LLUnop _ _ _ _ _ => False
+  | LLBinop _ _ _ _ _ _ => False
   end.
 
 Section FUNCTION.
@@ -135,4 +200,105 @@ Section FUNCTION.
     | None => False
     | Some inst => Uses inst r
     end.
+
+  Definition SuccOf (n: node) (m: node): Prop :=
+    match f.(fn_insts) ! n with
+    | None => False
+    | Some inst => Succeeds inst m
+    end.
+
+  Definition TermAt (n: node): Prop :=
+    match f.(fn_insts) ! n with
+    | None => False
+    | Some inst => Terminator inst
+    end.
+
 End FUNCTION.
+
+Definition get_successors (i: inst) :=
+  match i with
+  | LLLd _ _ next => [next]
+  | LLSt _ _ next => [next]
+  | LLArg _ _ next => [next]
+  | LLInt8 _ _ next => [next]
+  | LLInt16 _ _ next => [next]
+  | LLInt32 _ _ next => [next]
+  | LLInt64 _ _ next => [next]
+  | LLFrame _ _ next => [next]
+  | LLGlobal _ _ next => [next]
+  | LLExtern _ next => [next]
+  | LLInvoke _ _ _ next (Some exn) => [next; exn]
+  | LLInvoke _ _ _ next _ => [next]
+  | LLJcc _ bt bf => [bt; bf]
+  | LLJmp target => [target]
+  | LLUndef _ _ next => [next]
+  | LLUnop _ _ _ _ next => [next]
+  | LLBinop _ _ _ _ _ next => [next]
+  | _ => []
+  end.
+
+Lemma get_successors_correct:
+  forall (i: inst) (succ: node),
+    In succ (get_successors i) <-> Succeeds i succ.
+Proof.
+  split.
+  {
+    intros Hin.
+    unfold get_successors in Hin.
+    unfold Succeeds.
+    destruct i; try destruct exn;
+    repeat (destruct Hin; destruct H; subst; try inversion H; auto).
+  }
+  {
+    intros Hsucc.
+    unfold Succeeds in Hsucc.
+    unfold get_successors.
+    destruct i; try destruct exn; 
+    try destruct Hsucc; try inversion H; subst; simpl; auto.
+  }
+Qed.
+
+Definition get_predecessors (f: func) (n: node) :=
+  PTrie.values 
+    (PTrie.map_opt (fun k v => 
+      let succs := get_successors v in
+      if List.existsb (fun succ => Pos.eqb succ n) succs then Some k else None
+    ) f.(fn_insts)).
+
+Lemma get_predecessors_correct:
+  forall (f: func) (n: node) (pred: node),
+    In pred (get_predecessors f n) -> SuccOf f pred n.
+Proof.
+  intros f n pred.
+  intros Hin.
+  unfold get_predecessors in Hin. unfold SuccOf. unfold Succeeds.
+  apply PTrie.values_inversion in Hin.
+  destruct Hin as [k Hin].
+  apply PTrie.map_opt_inversion in Hin.
+  destruct Hin as [inst [Hinst Hpred]].
+  unfold get_successors in Hpred. unfold existsb in Hpred.
+  destruct inst; repeat match goal with
+    | [ H: Pos.eqb ?v n = false |- _ ] =>
+      clear H;
+      simpl in *
+    | [ H: Pos.eqb ?v n = true |- _ ] =>
+      apply Pos.eqb_eq in H;
+      subst n; 
+      simpl in Hpred;
+      inversion Hpred;
+      subst pred;
+      rewrite <- Hinst;
+      auto
+    | [ H: context [ Pos.eqb ?v n ] |- _ ] =>
+      destruct (Pos.eqb v n) eqn:E
+    | [ H: Some ?v = None |- _ ] =>
+      inversion H
+    | [ H: context [ LLInvoke _ _ _ _ ?exn ] |- _ ] =>
+      match exn with
+      | context [ None ] => simpl
+      | context [ Some ] => simpl
+      | _ => destruct exn
+      end
+    end.
+Qed.
+
