Export.v
@@ -1,0 +1,118 @@
+(* This file is part of the LLIR Semantics project. *)
+(* Licensing information is available in the LICENSE file. *)
+(* (C) 2020 Nandor Licker. All rights reserved. *)
+
+Require Import Coq.ZArith.ZArith.
+Require Import Coq.Lists.List.
+
+Require Import LLIR.LLIR.
+Require Import LLIR.Maps.
+Require Import LLIR.Dom.
+
+Ltac inversion_proof fn :=
+  intros inst n Heq;
+  unfold fn in Heq; unfold fn_insts in Heq;
+  repeat rewrite PTrie.set_get in Heq;
+  unfold fst in Heq; unfold snd in Heq;
+  repeat match goal with
+  | [ Heq: context [Pos.eqb ?v n] |- _ ] =>
+    destruct (Pos.eqb v n) eqn:E;
+    [ left; apply Pos.eqb_eq in E; subst n; split; auto | clear E; right]
+  end;
+  auto.
+
+Ltac defined_at_proof inv fn :=
+  intros n r Hdef_at;
+  unfold DefinedAt in *;
+  unfold Defs in *;
+  destruct ((fn_insts fn) ! n) eqn:Edef; try inversion Hdef_at;
+  apply inv in Edef;
+  repeat (destruct Edef as [Hdef|Edef]; try destruct Hdef as [Hi Hinst];
+    [ try left;
+      inversion Hinst as [Hinst_i]; rewrite <- Hinst_i in *;
+      match goal with
+      | [ Hi: ?v = n |- context [ ?v = n ] ] =>
+        subst r; subst n; auto
+      | [ H: False |- _ ] =>
+        inversion H
+      end
+    | match goal with
+      | [ H: context [ ?v = n ] |- (?v = n /\ _) \/ _ ] =>
+        auto
+      | _ =>
+        try right
+      end
+    ]);
+  inversion Edef.
+
+Ltac defs_are_unique_proof inv :=
+  intros def def' r Hdef Hdef';
+  apply inv in Hdef;
+  apply inv in Hdef';
+  repeat destruct Hdef as [Hd|Hdef]; repeat destruct Hdef' as [Hd'|Hdef'];
+  repeat match goal with
+  | [ H: ?v = ?def /\ ?v = r |- _ ] => destruct H; subst def
+  | [ |- ?v = ?v ] => reflexivity
+  | [ |- _ ] => subst r; auto
+  end.
+
+Ltac used_at_inversion_proof fn inv :=
+  intros n r Hused_at;
+  unfold UsedAt in *;
+  unfold Uses in *;
+  destruct ((fn_insts fn) ! n) eqn:Edef; try inversion Hused_at;
+  apply inv in Edef;
+  repeat match goal with
+  | [ H: ?v = n /\ Some ?inst = Some ?name |- _ ] =>
+    destruct H as [Hn Hinst];
+    inversion Hinst;
+    subst name
+  | [ H: False |- _ ] => inversion H
+  | [ H: ?a \/ ?b |- _ ] => destruct H
+  end;
+  match goal with
+  | [ Hn: ?vn = n, Hr: ?vr = r |- _] =>
+    assert (Hcase: vn = n /\ vr = r); [ split; [apply Hn|apply Hr] |]
+  | [ |- _ ] => simpl
+  end;
+  repeat match goal with
+  | [ H: ?vn = n /\ ?vr = r |- (?vn = n /\ ?vr = r) \/ _ ] => left; apply H
+  | [ H: ?vn = n /\ ?vr = r |- (?vn = n /\ ?vr = r) ] => apply H
+  | [ |- _ ] => right
+  end;
+  inversion H.
+
+Ltac reach_pred_step func pred :=
+  apply reach_succ with (a := pred);
+  [
+    unfold SuccOf;
+    simpl;
+    auto
+  |
+  ].
+
+Ltac block_elem_proof func func_inv p proof_prev :=
+  apply block_elem with (prev := p);
+  [ intro contra; inversion contra
+  | intro contra; inversion contra
+  | apply proof_prev
+  | unfold SuccOf; simpl; auto
+  | auto
+  | intros prev' Hsucc;
+    unfold SuccOf in Hsucc; unfold Succeeds in Hsucc;
+    remember ((fn_insts func) ! prev') as inst eqn:Hinst;
+    symmetry in Hinst;
+    apply func_inv in Hinst;
+    repeat destruct Hinst as [[Hl Hr]|Hinst]; subst inst; auto; try inversion Hsucc; try inversion H
+  ].
+
+Ltac block_header_proof func func_inv :=
+  right;
+  intros term Hsucc;
+  unfold SuccOf in Hsucc; unfold Succeeds in Hsucc; unfold TermAt;
+  remember ((fn_insts func) ! term) as inst eqn:H;
+  symmetry in H;
+  apply func_inv in H;
+  repeat destruct H as [[Hl Hr]|H];
+    subst inst; try subst term; simpl; auto;
+    inversion Hsucc; inversion H.
