SmallStep.v
@@ -1,0 +1,140 @@
+(* This file is part of the LLIR Semantics project. *)
+(* Licensing information is available in the LICENSE file. *)
+(* (C) 2020 Nandor Licker. All rights reserved. *)
+
+Require Import Values.
+Require Import LLIR.
+Require Import State.
+Require Import Maps.
+Require Import Coq.Lists.List.
+
+Import ListNotations.
+
+Inductive trace: Type.
+
+Inductive frame: Type :=
+  | Frame:
+    forall
+      (f: func)
+      (ret_pc: node)
+      (vregs: PTrie.t value),
+        frame.
+
+Definition stk_state := list frame.
+
+Axiom mem_state: Type.
+
+Inductive state: Type :=
+  | State:
+      forall
+        (stk: stk_state)
+        (mem: mem_state)
+        (pc: node),
+        state
+  .
+
+Definition get_inst (stk: stk_state) (pc: node): option inst :=
+  match stk with
+  | (Frame f _ _) :: _ => f.(fn_insts) ! pc
+  | _ => None
+  end.
+
+Axiom get_vreg: stk_state -> reg -> option value.
+
+Axiom set_vreg: stk_state -> reg -> value -> option stk_state.
+
+Axiom is_true: value -> Prop.
+
+Axiom is_false: value -> Prop.
+
+Axiom eval_unop: ty -> unop -> value -> option value.
+
+Axiom eval_binop: ty -> binop -> value -> value -> option value.
+
+Inductive step: state -> trace -> state -> Prop :=
+  | eval_jmp:
+    forall
+      (stk: stk_state) (mem: mem_state) (tr: trace)
+      (pc: node)
+      (target: node),
+      get_inst stk pc = Some (LLJmp target) ->
+      step
+        (State stk mem pc)
+        tr
+        (State stk mem target)
+  | eval_jcc_true:
+    forall
+      (stk: stk_state) (mem: mem_state) (tr: trace)
+      (pc: node)
+      (cond: reg) (brancht: node) (branchf: node)
+      (v: value),
+      get_inst stk pc = Some (LLJcc cond brancht branchf) ->
+      get_vreg stk cond = Some v ->
+      is_true v ->
+      step
+        (State stk mem pc)
+        tr
+        (State stk mem brancht)
+  | eval_jcc_false:
+    forall
+      (stk: stk_state) (mem: mem_state) (tr: trace)
+      (pc: node)
+      (cond: reg) (brancht: node) (branchf: node)
+      (v: value),
+      get_inst stk pc = Some (LLJcc cond brancht branchf) ->
+      get_vreg stk cond = Some v ->
+      is_false v ->
+      step
+        (State stk mem pc)
+        tr
+        (State stk mem brancht)
+  | eval_unary:
+    forall
+      (stk: stk_state) (mem: mem_state) (tr: trace)
+      (pc: node)
+      (ty: ty) (op: unop) (arg: reg) (dst: reg) (next: node)
+      (arg_value: value) (dst_value: value)
+      (stk': stk_state),
+      get_inst stk pc = Some (LLUnop ty op arg dst next) ->
+      get_vreg stk arg = Some arg_value ->
+      eval_unop ty op arg_value = Some dst_value ->
+      set_vreg stk dst dst_value = Some stk' ->
+      step
+        (State stk mem pc)
+        tr
+        (State stk' mem next)
+  | eval_binary:
+    forall
+      (stk: stk_state) (mem: mem_state) (tr: trace)
+      (pc: node)
+      (ty: ty) (op: binop) (lhs: reg) (rhs: reg) (dst: reg) (next: node)
+      (lhs_value: value) (rhs_value: value) (dst_value: value)
+      (stk': stk_state),
+      get_inst stk pc = Some (LLBinop ty op lhs rhs dst next) ->
+      get_vreg stk lhs = Some lhs_value ->
+      get_vreg stk rhs = Some rhs_value ->
+      eval_binop ty op lhs_value rhs_value = Some dst_value ->
+      set_vreg stk dst dst_value = Some stk' ->
+      step
+        (State stk mem pc)
+        tr
+        (State stk' mem next)
+  .
+
+  (*
+  | LLConst (value: qword) (dst: reg) (next: node)
+
+  | LLLd (addr: reg) (dst: reg) (next: node)
+  | LLSt (addr: reg) (val: reg) (next: node)
+
+  | LLArg (index: positive) (dst: reg) (next: node)
+
+  | LLFrame (object: positive) (dst: reg) (next: node)
+  | LLGlobal (object: positive) (dst: reg) (next: node)
+  | LLExtern (id: positive) (next: node)
+
+  | LLCall (callee: reg) (args: list reg) (dst: reg) (next: node)
+  | LLInvoke (callee: reg) (args: list reg) (dst: reg) (next: node) (exn: node)
+
+  | LLRet (value: reg)
+  *)
