test/fibonacci.v
@@ -1,0 +1,252 @@
+Require Import Coq.ZArith.ZArith.
+Require Import LLIR.LLIR.
+Require Import LLIR.Maps.
+Require Import LLIR.Values.
+Require Import LLIR.Verify.
+Require Import LLIR.State.
+Require Import LLIR.Export.
+Require Import LLIR.Dom.
+Require Import Coq.Lists.List.
+Import ListNotations.
+
+Definition fib: func := 
+  {| fn_stack :=
+    << >>
+  ; fn_insts :=
+    << (1%positive, LLArg 0 1%positive 2%positive)
+    ;  (2%positive, LLInt32 (((((O, O), (O, O)), ((O, O), (O, O))), (((O, O), (O, O)), ((O, O), (O, O)))), ((((O, O), (O, O)), ((O, O), (O, O))), (((O, O), (O, O)), ((O, O), (O, O))))) 2%positive 3%positive)
+    ;  (3%positive, LLInt32 (((((O, O), (O, O)), ((O, O), (O, O))), (((O, O), (O, O)), ((O, O), (O, O)))), ((((O, O), (O, O)), ((O, O), (O, O))), (((O, O), (O, O)), ((O, O), (O, I))))) 3%positive 4%positive)
+    ;  (4%positive, LLBinop I8 LLCmp 1%positive 2%positive 4%positive 5%positive)
+    ;  (5%positive, LLJcc 4%positive 17%positive 6%positive)
+    ;  (6%positive, LLInt32 (((((I, I), (I, I)), ((I, I), (I, I))), (((I, I), (I, I)), ((I, I), (I, I)))), ((((I, I), (I, I)), ((I, I), (I, I))), (((I, I), (I, I)), ((I, I), (I, I))))) 6%positive 7%positive)
+    ;  (7%positive, LLInt32 (((((O, O), (O, O)), ((O, O), (O, O))), (((O, O), (O, O)), ((O, O), (O, O)))), ((((O, O), (O, O)), ((O, O), (O, O))), (((O, O), (O, O)), ((O, O), (O, O))))) 7%positive 8%positive)
+    ;  (8%positive, LLJmp 12%positive)
+    ;  (12%positive, LLBinop I32 LLAdd 9%positive 11%positive 12%positive 13%positive)
+    ;  (13%positive, LLBinop I32 LLAdd 10%positive 6%positive 13%positive 14%positive)
+    ;  (14%positive, LLBinop I8 LLCmp 13%positive 2%positive 14%positive 15%positive)
+    ;  (15%positive, LLJcc 14%positive 12%positive 17%positive)
+    ;  (17%positive, LLRet 16%positive)
+    >>
+  ; fn_phis := 
+    << (12%positive
+       , [ LLPhi
+           [ (8%positive, 3%positive)
+           ; (15%positive, 12%positive)
+           ]
+           9%positive
+         ; LLPhi
+           [ (8%positive, 1%positive)
+           ; (15%positive, 13%positive)
+           ]
+           10%positive
+         ; LLPhi
+           [ (8%positive, 7%positive)
+           ; (15%positive, 9%positive)
+           ]
+           11%positive
+         ]
+       )
+    ;  (17%positive
+       , [ LLPhi
+           [ (5%positive, 3%positive)
+           ; (15%positive, 12%positive)
+           ]
+           16%positive
+         ]
+       )
+    >>
+  ; fn_entry := 1%positive
+  |}.
+
+Theorem fib_inversion:
+  forall (inst: option inst) (n: node),
+  (fn_insts fib) ! n = inst ->
+    (1%positive = n /\ Some (LLArg 0 1%positive 2%positive) = inst)
+    \/
+    (2%positive = n /\ Some (LLInt32 (((((O, O), (O, O)), ((O, O), (O, O))), (((O, O), (O, O)), ((O, O), (O, O)))), ((((O, O), (O, O)), ((O, O), (O, O))), (((O, O), (O, O)), ((O, O), (O, O))))) 2%positive 3%positive) = inst)
+    \/
+    (3%positive = n /\ Some (LLInt32 (((((O, O), (O, O)), ((O, O), (O, O))), (((O, O), (O, O)), ((O, O), (O, O)))), ((((O, O), (O, O)), ((O, O), (O, O))), (((O, O), (O, O)), ((O, O), (O, I))))) 3%positive 4%positive) = inst)
+    \/
+    (4%positive = n /\ Some (LLBinop I8 LLCmp 1%positive 2%positive 4%positive 5%positive) = inst)
+    \/
+    (5%positive = n /\ Some (LLJcc 4%positive 17%positive 6%positive) = inst)
+    \/
+    (6%positive = n /\ Some (LLInt32 (((((I, I), (I, I)), ((I, I), (I, I))), (((I, I), (I, I)), ((I, I), (I, I)))), ((((I, I), (I, I)), ((I, I), (I, I))), (((I, I), (I, I)), ((I, I), (I, I))))) 6%positive 7%positive) = inst)
+    \/
+    (7%positive = n /\ Some (LLInt32 (((((O, O), (O, O)), ((O, O), (O, O))), (((O, O), (O, O)), ((O, O), (O, O)))), ((((O, O), (O, O)), ((O, O), (O, O))), (((O, O), (O, O)), ((O, O), (O, O))))) 7%positive 8%positive) = inst)
+    \/
+    (8%positive = n /\ Some (LLJmp 12%positive) = inst)
+    \/
+    (12%positive = n /\ Some (LLBinop I32 LLAdd 9%positive 11%positive 12%positive 13%positive) = inst)
+    \/
+    (13%positive = n /\ Some (LLBinop I32 LLAdd 10%positive 6%positive 13%positive 14%positive) = inst)
+    \/
+    (14%positive = n /\ Some (LLBinop I8 LLCmp 13%positive 2%positive 14%positive 15%positive) = inst)
+    \/
+    (15%positive = n /\ Some (LLJcc 14%positive 12%positive 17%positive) = inst)
+    \/
+    (17%positive = n /\ Some (LLRet 16%positive) = inst)
+    \/
+    inst = None.
+Proof. inversion_proof fib. Qed.
+
+Theorem fib_defined_at_inversion:
+  forall (n: node) (r: reg),
+    DefinedAt fib n r -> 
+      (1%positive = n /\ 1%positive = r)
+      \/
+      (2%positive = n /\ 2%positive = r)
+      \/
+      (3%positive = n /\ 3%positive = r)
+      \/
+      (4%positive = n /\ 4%positive = r)
+      \/
+      (6%positive = n /\ 6%positive = r)
+      \/
+      (7%positive = n /\ 7%positive = r)
+      \/
+      (12%positive = n /\ 12%positive = r)
+      \/
+      (13%positive = n /\ 13%positive = r)
+      \/
+      (14%positive = n /\ 14%positive = r).
+Proof. defined_at_proof fib_inversion fib. Qed.
+
+Theorem fib_used_at_inversion:
+  forall (n: node) (r: reg),
+    UsedAt fib n r -> 
+      (4%positive = n /\ 1%positive = r)
+      \/
+      (4%positive = n /\ 2%positive = r)
+      \/
+      (5%positive = n /\ 4%positive = r)
+      \/
+      (9%positive = n /\ 3%positive = r)
+      \/
+      (9%positive = n /\ 12%positive = r)
+      \/
+      (10%positive = n /\ 1%positive = r)
+      \/
+      (10%positive = n /\ 13%positive = r)
+      \/
+      (11%positive = n /\ 7%positive = r)
+      \/
+      (11%positive = n /\ 9%positive = r)
+      \/
+      (12%positive = n /\ 9%positive = r)
+      \/
+      (12%positive = n /\ 11%positive = r)
+      \/
+      (13%positive = n /\ 10%positive = r)
+      \/
+      (13%positive = n /\ 6%positive = r)
+      \/
+      (14%positive = n /\ 13%positive = r)
+      \/
+      (14%positive = n /\ 2%positive = r)
+      \/
+      (15%positive = n /\ 14%positive = r)
+      \/
+      (16%positive = n /\ 3%positive = r)
+      \/
+      (16%positive = n /\ 12%positive = r)
+      \/
+      (17%positive = n /\ 16%positive = r).
+Proof. used_at_inversion_proof fib fib_inversion. Qed.
+
+Theorem fib_defs_are_unique: defs_are_unique fib.
+Proof. defs_are_unique_proof fib_defined_at_inversion. Qed.
+
+Theorem fib_reach_1: Reachable fib 1%positive. Proof. apply reach_entry. Qed.
+Theorem fib_reach_2: Reachable fib 2%positive. Proof. reach_pred_step fib 1%positive. apply fib_reach_1. Qed.
+Theorem fib_reach_3: Reachable fib 3%positive. Proof. reach_pred_step fib 2%positive. apply fib_reach_2. Qed.
+Theorem fib_reach_4: Reachable fib 4%positive. Proof. reach_pred_step fib 3%positive. apply fib_reach_3. Qed.
+Theorem fib_reach_5: Reachable fib 5%positive. Proof. reach_pred_step fib 4%positive. apply fib_reach_4. Qed.
+Theorem fib_reach_6: Reachable fib 6%positive. Proof. reach_pred_step fib 5%positive. apply fib_reach_5. Qed.
+Theorem fib_reach_7: Reachable fib 7%positive. Proof. reach_pred_step fib 6%positive. apply fib_reach_6. Qed.
+Theorem fib_reach_8: Reachable fib 8%positive. Proof. reach_pred_step fib 7%positive. apply fib_reach_7. Qed.
+Theorem fib_reach_12: Reachable fib 12%positive. Proof. reach_pred_step fib 8%positive. apply fib_reach_8. Qed.
+Theorem fib_reach_13: Reachable fib 13%positive. Proof. reach_pred_step fib 12%positive. apply fib_reach_12. Qed.
+Theorem fib_reach_14: Reachable fib 14%positive. Proof. reach_pred_step fib 13%positive. apply fib_reach_13. Qed.
+Theorem fib_reach_15: Reachable fib 15%positive. Proof. reach_pred_step fib 14%positive. apply fib_reach_14. Qed.
+Theorem fib_reach_17: Reachable fib 17%positive. Proof. reach_pred_step fib 15%positive. apply fib_reach_15. Qed.
+
+Theorem fib_bb_1: BasicBlock fib 1%positive 1%positive.
+Proof.
+  apply block_header.
+  apply fib_reach_1.
+auto.
+Qed.
+
+Theorem fib_bb_2: BasicBlock fib 1%positive 2%positive.
+Proof.
+  block_elem_proof fib fib_inversion 1%positive fib_bb_1.
+Qed.
+
+Theorem fib_bb_3: BasicBlock fib 1%positive 3%positive.
+Proof.
+  block_elem_proof fib fib_inversion 2%positive fib_bb_2.
+Qed.
+
+Theorem fib_bb_4: BasicBlock fib 1%positive 4%positive.
+Proof.
+  block_elem_proof fib fib_inversion 3%positive fib_bb_3.
+Qed.
+
+Theorem fib_bb_5: BasicBlock fib 1%positive 5%positive.
+Proof.
+  block_elem_proof fib fib_inversion 4%positive fib_bb_4.
+Qed.
+
+Theorem fib_bb_6: BasicBlock fib 6%positive 6%positive.
+Proof.
+  apply block_header.
+  apply fib_reach_6.
+  block_header_proof fib fib_inversion.
+Qed.
+
+Theorem fib_bb_7: BasicBlock fib 6%positive 7%positive.
+Proof.
+  block_elem_proof fib fib_inversion 6%positive fib_bb_6.
+Qed.
+
+Theorem fib_bb_8: BasicBlock fib 6%positive 8%positive.
+Proof.
+  block_elem_proof fib fib_inversion 7%positive fib_bb_7.
+Qed.
+
+Theorem fib_bb_12: BasicBlock fib 12%positive 12%positive.
+Proof.
+  apply block_header.
+  apply fib_reach_12.
+  block_header_proof fib fib_inversion.
+Qed.
+
+Theorem fib_bb_13: BasicBlock fib 12%positive 13%positive.
+Proof.
+  block_elem_proof fib fib_inversion 12%positive fib_bb_12.
+Qed.
+
+Theorem fib_bb_14: BasicBlock fib 12%positive 14%positive.
+Proof.
+  block_elem_proof fib fib_inversion 13%positive fib_bb_13.
+Qed.
+
+Theorem fib_bb_15: BasicBlock fib 12%positive 15%positive.
+Proof.
+  block_elem_proof fib fib_inversion 14%positive fib_bb_14.
+Qed.
+
+Theorem fib_bb_17: BasicBlock fib 17%positive 17%positive.
+Proof.
+  apply block_header.
+  apply fib_reach_17.
+  block_header_proof fib fib_inversion.
+Qed.
+
+Theorem fib_bb_dom_tree:
+  Dominates fib 5%positive 17%positive
+  \/
+  Dominates fib 5%positive 6%positive.
+Admitted.
+
